x86/Symbtablegenproof1.v
@@ -15,11 +15,9 @@ Require Import Linking.
 Require Globalenvs.
 Import ListNotations.
 
-(***** Remove Proofs By Chris Start ******)
-(*
-Lemma get_symbentry_pres_internal_prop : forall did cid id dsz csz def,
+Lemma get_symbentry_pres_internal_prop : forall rdid did cid id rdsz dsz csz def,
     is_def_internal is_fundef_internal def = 
-    is_symbentry_internal (get_symbentry did cid dsz csz id def).
+    is_symbentry_internal (get_symbentry rdid did cid rdsz dsz csz id def).
 Proof.
   intros. destruct def.
   destruct g. destruct f.
@@ -27,48 +25,80 @@ Proof.
   - cbn. auto.
   - cbn. unfold is_var_internal. 
     destruct (gvar_init v); cbn; auto.
+    destruct (gvar_readonly v); cbn; auto.
+    destruct i; cbn; auto.
+    destruct l; cbn; auto.
     destruct i; cbn; auto.
     destruct l; cbn; auto.
   - cbn. auto.
 Qed.
 
 
-Lemma get_symbentry_id : forall d_id c_id dsz csz id def,
-    symbentry_id (get_symbentry d_id c_id dsz csz id def) = id.
+Lemma get_symbentry_id : forall rd_id d_id c_id rdsz dsz csz id def,
+    symbentry_id (get_symbentry rd_id d_id c_id rdsz dsz csz id def) = id.
 Proof.
   intros until def.
   destruct def. destruct g. destruct f.
   simpl; auto.
   simpl; auto.
-  simpl. destruct (gvar_init v); auto. destruct i; auto. destruct l; auto.
+  simpl. destruct (gvar_init v); destruct (gvar_readonly v); auto.
+  destruct i; auto. destruct l; auto.
+  destruct i; auto. destruct l; auto.  
   simpl; auto.
 Qed.
 
 
 Lemma get_symbentry_eq_id_inv: 
-  forall did1 cid1 dsz1 csz1 id1 def1 did2 cid2 dsz2 csz2 id2 def2,
-    get_symbentry did1 cid1 dsz1 csz1 id1 def1 = get_symbentry did2 cid2 dsz2 csz2 id2 def2 -> id1 = id2.
+  forall rdid1 did1 cid1 rdsz1 dsz1 csz1 id1 def1 rdid2 did2 cid2 rdsz2 dsz2 csz2 id2 def2,
+    get_symbentry rdid1 did1 cid1 rdsz1 dsz1 csz1 id1 def1 = get_symbentry rdid2 did2 cid2 rdsz2 dsz2 csz2 id2 def2 -> id1 = id2.
 Proof.
   intros. 
-  generalize (get_symbentry_id did1 cid1 dsz1 csz1 id1 def1).
+  generalize (get_symbentry_id rdid1 did1 cid1 rdsz1 dsz1 csz1 id1 def1).
   intros ID1.
-  generalize (get_symbentry_id did2 cid2 dsz2 csz2 id2 def2).
+  generalize (get_symbentry_id rdid2 did2 cid2 rdsz2 dsz2 csz2 id2 def2).
   intros ID2.
   rewrite H in ID1.
   rewrite ID1 in ID2.
   inv ID2. auto.
 Qed.
 
-Lemma get_var_entry_size : forall did cid dsz csz id v, 
-    symbentry_size (get_symbentry did cid dsz csz id (Some (Gvar v))) = AST.init_data_list_size (gvar_init v).
+Lemma get_var_entry_size : forall rdid did cid rdsz dsz csz id v, 
+    symbentry_size (get_symbentry rdid did cid rdsz dsz csz id (Some (Gvar v))) = AST.init_data_list_size (gvar_init v).
 Proof.
   intros.
-  cbn. destruct (gvar_init v); auto.
+  cbn. destruct (gvar_init v); destruct (gvar_readonly v); auto.
+  destruct i; auto.
+  destruct l; auto.
+  cbn. omega.
   destruct i; auto.
   destruct l; auto.
   cbn. omega.
 Qed.
 
+Lemma acc_init_rodata_app : forall def l1 l2,
+    (acc_init_rodata def l1) ++ l2 = acc_init_rodata def (l1 ++ l2).
+Proof.
+  intros def l1 l2. destruct def as (id & def').
+  simpl. rewrite app_assoc. auto.
+Qed.
+
+Lemma fold_right_acc_init_rodata_app' : forall defs l,
+    fold_right acc_init_rodata [] defs ++ l = fold_right acc_init_rodata l defs.
+Proof.
+  induction defs. 
+  - intros l. simpl. auto.
+  - intros l. simpl. 
+    rewrite acc_init_rodata_app. rewrite IHdefs. auto.
+Qed.
+
+Lemma fold_right_acc_init_rodata_app : forall defs1 defs2,
+    fold_right acc_init_rodata [] (defs1 ++ defs2) = 
+    fold_right acc_init_rodata [] defs1 ++ fold_right acc_init_rodata [] defs2.
+Proof.
+  intros.
+  rewrite fold_right_app.
+  rewrite <- fold_right_acc_init_rodata_app'. auto.
+Qed.
 
 Lemma acc_init_data_app : forall def l1 l2,
     (acc_init_data def l1) ++ l2 = acc_init_data def (l1 ++ l2).
@@ -119,85 +149,93 @@ Proof.
   rewrite <- fold_right_acc_instrs_app'. auto.
 Qed.
 
-Lemma update_code_data_size_eq : forall def dsz csz dincr cincr,
+Lemma update_section_size_eq : forall id def rdsz dsz csz rdincr dincr cincr,
+    rdincr = init_data_list_size (get_def_init_rodata def) ->
     dincr = init_data_list_size (get_def_init_data def) ->
     cincr = code_size (get_def_instrs def) ->
-    update_code_data_size dsz csz def = (dincr + dsz, cincr + csz).
+    update_section_size rdsz dsz csz id def = (rdincr + rdsz, dincr + dsz, cincr + csz).
 Proof.
-  intros def dsz csz dincr cincr DINCR CINCR.
-  unfold update_code_data_size. destruct def. destruct g. destruct f.
+  intros id def rdsz dsz csz rdincr dincr cincr RDINCR DINCR CINCR.
+  unfold update_section_size. destruct def. destruct g. destruct f.
   - simpl in *. subst. f_equal; omega.
   - simpl in *. subst. f_equal; omega.
-  - simpl in DINCR, CINCR. subst.
-    destruct (gvar_init v).
-    + simpl. auto.
-    + destruct i; try (f_equal; omega).
-      destruct l; f_equal; omega.
+  - simpl in RDINCR, DINCR, CINCR. subst.
+    destruct (gvar_init v); destruct (gvar_readonly v);
+      try(simpl; auto); try (destruct i; try (f_equal; omega);
+      destruct l; f_equal; rewrite Z.add_comm; auto).
   - simpl in *. subst. f_equal; omega.
 Qed.
 
-Lemma acc_symb_size: forall d_id c_id defs s1 s2 dsz1 csz1 dsz2 csz2 data code,
-    fold_left (acc_symb d_id c_id) defs (s1, dsz1, csz1) = (s2, dsz2, csz2) ->
+Lemma acc_symb_size: forall rd_id d_id c_id defs s1 s2 rdsz1 dsz1 csz1 rdsz2 dsz2 csz2 rodata data code,
+    fold_left (acc_symb rd_id d_id c_id) defs (s1, rdsz1, dsz1, csz1) = (s2, rdsz2, dsz2, csz2) ->
+    init_data_list_size rodata = rdsz1 ->
     init_data_list_size data = dsz1 ->
     code_size code = csz1 ->
-    init_data_list_size (fold_right acc_init_data data defs) = dsz2 /\ 
+    init_data_list_size (fold_right acc_init_rodata rodata defs) = rdsz2 /\
+    init_data_list_size (fold_right acc_init_data data defs) = dsz2 /\
     code_size (fold_right acc_instrs code defs) = csz2.
 Proof.
   induction defs as [| def defs].
-  - intros s1 s2 dsz1 csz1 dsz2 csz2 data code SYMB INIT CODE.
+  - intros s1 s2 rdsz1 dsz1 csz1 rdsz2 dsz2 csz2 rodata data code SYMB INITRD INITD CODE.
     simpl in *. inv SYMB. auto.
-  - intros s1 s2 dsz1 csz1 dsz2 csz2 data code SYMB INIT CODE.
+  - intros s1 s2 rdsz1 dsz1 csz1 rdsz2 dsz2 csz2 rodata data code SYMB INITRD INITD CODE.
     destruct def as (id, def).
     simpl in *. destr_in SYMB.
     rewrite init_data_list_size_app.
+    rewrite init_data_list_size_app.
     rewrite code_size_app.
-    erewrite update_code_data_size_eq in Heqp; eauto.
+    erewrite update_section_size_eq in Heqp; eauto.
     inv Heqp.
     rewrite <- init_data_list_size_app in SYMB.
+    rewrite <- init_data_list_size_app in SYMB.
     rewrite <- code_size_app in SYMB.
-    generalize (IHdefs _ _ _ _ _ _ _ _ SYMB 
+    generalize (IHdefs _ _ _ _ _ _ _ _ _ _ _ SYMB
+                       (@eq_refl _ (init_data_list_size (get_def_init_rodata def ++ rodata)))
                        (@eq_refl _ (init_data_list_size (get_def_init_data def ++ data)))
                        (@eq_refl _ (code_size (get_def_instrs def ++ code)))).
-    destruct 1. subst. split.
-    + rewrite <- (fold_right_acc_init_data_app' defs data).
+    destruct 1. destruct H0. subst. split.
+    + rewrite <- (fold_right_acc_init_rodata_app' defs rodata).
+      rewrite <- (fold_right_acc_init_rodata_app' defs (get_def_init_rodata def ++ rodata)).
+      repeat rewrite init_data_list_size_app.
+      omega.
+    + split. subst. rewrite <- (fold_right_acc_init_data_app' defs data).
       rewrite <- (fold_right_acc_init_data_app' defs (get_def_init_data def ++ data)).
       repeat rewrite init_data_list_size_app.
       omega.
-    + rewrite <- (fold_right_acc_instrs_app' defs code).
+      rewrite <- (fold_right_acc_instrs_app' defs code).
       rewrite <- (fold_right_acc_instrs_app' defs (get_def_instrs def ++ code)).
       repeat rewrite code_size_app.
       omega.
 Qed.
 
-
-Lemma gen_symb_table_size: forall defs d_id c_id stbl dsz csz,
-    gen_symb_table d_id c_id defs = (stbl, dsz, csz) ->
+Lemma gen_symb_table_size: forall defs rd_id d_id c_id stbl rdsz dsz csz,
+    gen_symb_table rd_id d_id c_id defs = (stbl, rdsz, dsz, csz) ->
+    sec_size (create_rodata_section defs) = rdsz /\
     sec_size (create_data_section defs) = dsz /\
     sec_size (create_code_section defs) = csz.
 Proof.
-  intros defs d_id c_id stbl dsz csz SGEN.
+  intros defs rd_id d_id c_id stbl rdsz dsz csz SGEN.
   simpl. unfold gen_symb_table in SGEN.
-  destr_in SGEN. destruct p. inv SGEN. 
-  eapply acc_symb_size; eauto.
+  destr_in SGEN. destruct p. destruct p. inv SGEN. 
+  eapply acc_symb_size; eauto. 
 Qed.
 
-
-Lemma acc_symb_append : forall d_id c_id defs dsz1 csz1 stbl1 dsz2 csz2 stbl2 stbl3,
-    fold_left (acc_symb d_id c_id) defs (stbl1, dsz1, csz1) = (stbl2, dsz2, csz2) ->
-    fold_left (acc_symb d_id c_id) defs (stbl1 ++ stbl3, dsz1, csz1) = (stbl2 ++ stbl3, dsz2, csz2).
+Lemma acc_symb_append : forall rd_id r_id c_id defs rdsz1 dsz1 csz1 stbl1 rdsz2 dsz2 csz2 stbl2 stbl3,
+    fold_left (acc_symb rd_id r_id c_id) defs (stbl1, rdsz1, dsz1, csz1) = (stbl2, rdsz2, dsz2, csz2) ->
+    fold_left (acc_symb rd_id r_id c_id) defs (stbl1 ++ stbl3, rdsz1, dsz1, csz1) = (stbl2 ++ stbl3, rdsz2, dsz2, csz2).
 Proof.
   induction defs.
   - intros until stbl2. intros stbl3 ACC. simpl in *.
     inv ACC. auto.
   - intros until stbl2. intros stbl3 ACC. simpl in *.
-    destr_in ACC. destruct a. inv Heqp. destr_in ACC.
+    destr_in ACC. destruct a. inv Heqp. destr_in ACC. destruct p.
     rewrite app_comm_cons.
     apply IHdefs. auto.
 Qed.
 
-Lemma acc_symb_append_nil : forall d_id c_id defs dsz1 csz1 dsz2 csz2 stbl2 stbl3,
-    fold_left (acc_symb d_id c_id) defs ([], dsz1, csz1) = (stbl2, dsz2, csz2) ->
-    fold_left (acc_symb d_id c_id) defs (stbl3, dsz1, csz1) = (stbl2 ++ stbl3, dsz2, csz2).
+Lemma acc_symb_append_nil : forall rd_id r_id c_id defs rdsz1 dsz1 csz1 rdsz2 dsz2 csz2 stbl2 stbl3,
+    fold_left (acc_symb rd_id r_id c_id) defs ([], rdsz1, dsz1, csz1) = (stbl2, rdsz2, dsz2, csz2) ->
+    fold_left (acc_symb rd_id r_id c_id) defs (stbl3, rdsz1, dsz1, csz1) = (stbl2 ++ stbl3, rdsz2, dsz2, csz2).
 Proof.
   intros until stbl3. intros ACC.
   replace stbl3 with ([] ++ stbl3) by auto.
@@ -205,20 +243,20 @@ Proof.
 Qed.
 
 
-Lemma acc_symb_inv: forall asf d_id c_id defs stbl1 dsz1 csz1 stbl2 dsz2 csz2,
-    asf = (acc_symb d_id c_id) ->
-    fold_left asf defs (stbl1, dsz1, csz1) = (stbl2, dsz2, csz2) ->
+Lemma acc_symb_inv: forall asf rd_id r_id c_id defs stbl1 rdsz1 dsz1 csz1 stbl2 rdsz2 dsz2 csz2,
+    asf = (acc_symb rd_id r_id c_id) ->
+    fold_left asf defs (stbl1, rdsz1, dsz1, csz1) = (stbl2, rdsz2, dsz2, csz2) ->
     exists stbl1', stbl2 = stbl1' ++ stbl1 /\
-              fold_left asf defs ([], dsz1, csz1) = (stbl1', dsz2, csz2).
+              fold_left asf defs ([], rdsz1, dsz1, csz1) = (stbl1', rdsz2, dsz2, csz2).
 Proof.
   induction defs.
-  - intros stbl1 dsz1 csz1 stbl2 dsz2 csz2 ASF ACC.
+  - intros stbl1 rdsz1 dsz1 csz1 stbl2 rdsz2 dsz2 csz2 ASF ACC.
     simpl in *. inv ACC. exists nil. eauto.
   - intros until csz2. intros ASF ACC. simpl in *.
     rewrite ASF in ACC. simpl in ACC. destruct a as (id & def).
-    destruct (update_code_data_size dsz1 csz1 def) as [dsize' csize'] eqn:UPDATE.
+    destruct (update_section_size rdsz1 dsz1 csz1 id def) as [dsize' csize'] eqn:UPDATE. destruct dsize'.
     rewrite <- ASF in ACC.
-    generalize (IHdefs _ _ _ _ _ _ ASF ACC).
+    generalize (IHdefs _ _ _ _ _ _ _ _ ASF ACC).
     destruct 1 as (stbl1' & EQ & ACC1).
     rewrite app_cons_comm in EQ.
     rewrite EQ.
@@ -228,10 +266,10 @@ Proof.
     apply acc_symb_append_nil. auto.
 Qed.
 
-Lemma acc_symb_inv': forall d_id c_id defs stbl1 dsz1 csz1 stbl2 dsz2 csz2,
-    fold_left (acc_symb d_id c_id) defs (stbl1, dsz1, csz1) = (stbl2, dsz2, csz2) ->
+Lemma acc_symb_inv': forall rd_id r_id c_id defs stbl1 rdsz1 dsz1 csz1 stbl2 rdsz2 dsz2 csz2,
+    fold_left (acc_symb rd_id r_id c_id) defs (stbl1, rdsz1, dsz1, csz1) = (stbl2, rdsz2, dsz2, csz2) ->
     exists stbl1', stbl2 = stbl1' ++ stbl1 /\
-              fold_left (acc_symb d_id c_id) defs ([], dsz1, csz1) = (stbl1', dsz2, csz2).
+              fold_left (acc_symb rd_id r_id c_id) defs ([], rdsz1, dsz1, csz1) = (stbl1', rdsz2, dsz2, csz2).
 Proof.
   intros. eapply acc_symb_inv; eauto.
 Qed.
@@ -245,32 +283,33 @@ Definition symbentry_index_in_range range e :=
 Definition symbtable_indexes_in_range range t :=
   Forall (symbentry_index_in_range range) t.
 
-Lemma get_symbentry_in_range: forall d_id c_id dsz csz id def,
-  symbentry_index_in_range [d_id; c_id] (get_symbentry d_id c_id dsz csz id def).
+Lemma get_symbentry_in_range: forall rd_id r_id c_id rdsz dsz csz id def,
+  symbentry_index_in_range [rd_id; r_id; c_id] (get_symbentry rd_id r_id c_id rdsz dsz csz id def).
 Proof.
   intros.
   destruct def. destruct g. destruct f.
   - cbn. auto.
   - cbn. auto.
-  - cbn. destr; cbn; auto.
+  - cbn. destr; cbn; auto. destruct (gvar_readonly v);
     destruct i; cbn; auto.
+    destruct l; cbn; auto.
     destruct l; cbn; auto.
   - cbn. auto.
 Qed.
 
-Lemma acc_symb_index_in_range: forall d_id c_id defs dsz1 csz1 tbl dsz2 csz2,
-      fold_left (acc_symb d_id c_id) defs ([], dsz1, csz1) = (tbl, dsz2, csz2)
-      -> symbtable_indexes_in_range [d_id; c_id] (rev tbl).
+Lemma acc_symb_index_in_range: forall rd_id r_id c_id defs rdsz1 dsz1 csz1 tbl rdsz2 dsz2 csz2,
+      fold_left (acc_symb rd_id r_id c_id) defs ([], rdsz1, dsz1, csz1) = (tbl, rdsz2, dsz2, csz2)
+      -> symbtable_indexes_in_range [rd_id; r_id; c_id] (rev tbl).
 Proof.
   induction defs as [| def defs].
   - intros until csz2. intros ACC. cbn in *.
     inv ACC. red. cbn. apply Forall_nil.
   - intros until csz2. intros ACC. cbn in *.
-    destruct def as [id def]. destr_in ACC.
-    generalize (acc_symb_inv _ _ _ _ _ _ _ _ _ _ eq_refl ACC).
+    destruct def as [id def]. destr_in ACC. destruct p.
+    generalize (acc_symb_inv _ _ _ _ _ _ _ _ _ _ _ _ _ eq_refl ACC).
     destruct 1 as (stbl1' & EQ & ACC'). subst.
     rewrite rev_unit.
-    generalize (IHdefs _ _ _ _ _ ACC').
+    generalize (IHdefs _ _ _ _ _ _ _ ACC').
     intros IN_RNG.
     red. rewrite Forall_forall.
     intros x IN.
@@ -281,13 +320,13 @@ Proof.
       apply IN_RNG; auto.
 Qed.
 
-Lemma gen_symb_table_index_in_range : forall defs sec_data_id sec_code_id stbl dsz csz,
-    gen_symb_table sec_data_id sec_code_id defs = (stbl, dsz, csz) ->
-    symbtable_indexes_in_range [sec_data_id; sec_code_id] stbl.
+Lemma gen_symb_table_index_in_range : forall defs sec_rodata_id sec_data_id sec_code_id stbl rdsz dsz csz,
+    gen_symb_table sec_rodata_id sec_data_id sec_code_id defs = (stbl, rdsz, dsz, csz) ->
+    symbtable_indexes_in_range [sec_rodata_id; sec_data_id; sec_code_id] stbl.
 Proof.
   intros until csz.
   intros GS.
-  unfold gen_symb_table in GS. destr_in GS. destruct p. inv GS.
+  unfold gen_symb_table in GS. destr_in GS. destruct p. destruct p. inv GS.
   apply acc_symb_inv' in Heqp.
   destruct Heqp as (stbl1' & EQ & FL). subst.
   rewrite rev_app_distr. cbn.
@@ -296,67 +335,76 @@ Proof.
   auto.
 Qed.
 
-Lemma get_var_entry_type : forall did cid dsz1 csz1 id v,
-    symbentry_type (get_symbentry did cid dsz1 csz1 id (Some (Gvar v))) = symb_data.
+Lemma get_var_entry_type : forall rodid did cid rdsz1 dsz1 csz1 id v,
+    symbentry_type (get_symbentry rodid did cid rdsz1 dsz1 csz1 id (Some (Gvar v))) = symb_data.
 Proof.
   intros. cbn.
-  destruct (gvar_init v); auto.
+  destruct (gvar_init v); destruct (gvar_readonly v); auto.
+  destruct i; auto.
+  destruct l; auto.
   destruct i; auto.
   destruct l; auto.
 Qed.
 
-Lemma get_fun_entry_type : forall did cid dsz1 csz1 id f,
-    symbentry_type (get_symbentry did cid dsz1 csz1 id (Some (Gfun f))) = symb_func.
+Lemma get_fun_entry_type : forall rodid did cid rdsz1 dsz1 csz1 id f,
+    symbentry_type (get_symbentry rodid did cid rdsz1 dsz1 csz1 id (Some (Gfun f))) = symb_func.
 Proof.
   intros. cbn.
   destruct f; auto.
 Qed.
 
-Lemma get_none_entry_type : forall did cid dsz1 csz1 id,
-    symbentry_type (get_symbentry did cid dsz1 csz1 id None) = symb_notype.
+Lemma get_none_entry_type : forall rodid did cid rdsz1 dsz1 csz1 id,
+    symbentry_type (get_symbentry rodid did cid rdsz1 dsz1 csz1 id None) = symb_notype.
 Proof.
   intros. cbn. auto.
 Qed.
 
-Lemma get_none_entry_secindex : forall did cid dsz1 csz1 id,
-    symbentry_secindex (get_symbentry did cid dsz1 csz1 id None) = secindex_undef.
+Lemma get_none_entry_secindex : forall rodid did cid rdsz1 dsz1 csz1 id,
+    symbentry_secindex (get_symbentry rodid did cid rdsz1 dsz1 csz1 id None) = secindex_undef.
 Proof.
   intros. cbn. auto.
 Qed.
 
-Lemma get_symbentry_eq_gvar_init: forall did cid dsz1 csz1 id v1 v2,
+Lemma get_symbentry_eq_gvar_init_readonly: forall rodid did cid rdsz1 dsz1 csz1 id v1 v2,
     gvar_init v1 = gvar_init v2 ->
-    get_symbentry did cid dsz1 csz1 id (Some (Gvar v1)) = 
-    get_symbentry did cid dsz1 csz1 id (Some (Gvar v2)).
+    gvar_readonly v1 = gvar_readonly v2 ->
+    get_symbentry rodid did cid rdsz1 dsz1 csz1 id (Some (Gvar v1)) = 
+    get_symbentry rodid did cid rdsz1 dsz1 csz1 id (Some (Gvar v2)).
 Proof.
-  intros. cbn. rewrite H. auto.
+  intros. cbn. rewrite H. rewrite H0. auto.
 Qed.
 
-Lemma update_size_offset : forall def dsz csz dsz1 csz1 dofs cofs,
-    update_code_data_size dsz csz def = (dsz1, csz1) ->
-    update_code_data_size (dofs + dsz) (cofs + csz) def = (dofs + dsz1, cofs + csz1).
+Lemma update_size_offset : forall id def rdsz dsz csz rdsz1 dsz1 csz1 rdofs dofs cofs,
+    update_section_size rdsz dsz csz id def = (rdsz1, dsz1, csz1) ->
+    update_section_size (rdofs + rdsz) (dofs + dsz) (cofs + csz) id def = (rdofs + rdsz1, dofs + dsz1, cofs + csz1).
 Proof.
   intros until cofs. intros UPDATE.
   destruct def. destruct g. destruct f.
   - cbn in *. inv UPDATE. f_equal; omega.
   - cbn in *. inv UPDATE. f_equal; omega.
-  - unfold update_code_data_size in *.
-    destr_in UPDATE. 
-    destruct i; try (inv UPDATE; cbn; f_equal; omega).
-    destruct l; try (inv UPDATE; cbn; f_equal; omega).
+  - unfold update_section_size in *.
+    destruct (gvar_init v); destruct (gvar_readonly v).
+    inv UPDATE. reflexivity.
+    inv UPDATE. reflexivity.
+    destruct i; destruct l;
+      try (inv UPDATE; cbn; rewrite <- Z.add_assoc; reflexivity).    
+    inv UPDATE. reflexivity.
+    destruct i; destruct l;
+      try (inv UPDATE; cbn; rewrite <- Z.add_assoc; reflexivity).    
+    inv UPDATE. reflexivity.
   - cbn in *. inv UPDATE. auto.
 Qed.
 
-Lemma acc_symb_pres_ids: forall did cid defs dsz1 csz1 stbl2 dsz2 csz2,
-    fold_left (acc_symb did cid) defs ([], dsz1, csz1) = (stbl2, dsz2, csz2) ->
+Lemma acc_symb_pres_ids: forall rodid did cid defs rdsz1 dsz1 csz1 stbl2 rdsz2 dsz2 csz2,
+    fold_left (acc_symb rodid did cid) defs ([], rdsz1, dsz1, csz1) = (stbl2, rdsz2, dsz2, csz2) ->
     (map fst defs) = get_symbentry_ids (rev stbl2).
 Proof.
   induction defs as [| def defs].
   - cbn.  inversion 1. subst. inv H.
     cbn. auto.
-  - intros dsz1 csz1 stbl2 dsz2 csz2 FL.
+  - intros rdsz1 dsz1 csz1 stbl2 rdsz2 dsz2 csz2 FL.
     cbn in *. destruct def as (id, def).
-    destr_in FL. cbn.
+    destr_in FL. destruct p. cbn.
     apply acc_symb_inv' in FL. 
     destruct FL as (stbl2' & EQ & FL). subst.
     unfold get_symbentry_ids.
@@ -367,13 +415,13 @@ Proof.
     eapply IHdefs; eauto.
 Qed.
 
-Lemma gen_symb_table_pres_ids: forall did cid defs stbl dsz csz,
-    gen_symb_table did cid defs = (stbl, dsz, csz) ->
+Lemma gen_symb_table_pres_ids: forall rdid did cid defs stbl rdsz dsz csz,
+    gen_symb_table rdid did cid defs = (stbl, rdsz, dsz, csz) ->
     (map fst defs) = (get_symbentry_ids stbl).
 Proof.
-  intros did cid defs stbl dsz csz GST.
+  intros rdid did cid defs stbl rdsz dsz csz GST.
   unfold gen_symb_table in GST.
-  destr_in GST. destruct p. inv GST.
+  destr_in GST. destruct p. destruct p. inv GST.
   apply acc_symb_inv' in Heqp.
   destruct Heqp as (s' & EQ & FL). subst.
   rewrite rev_app_distr. cbn.
@@ -451,18 +499,30 @@ Proof.
   cbn. rewrite peq_true. cbn. auto.
 Qed.
 
+Definition def_rodata_size (def: option gdef) :=
+  init_data_list_size (get_def_init_rodata def).
+
 Definition def_data_size (def: option gdef) :=
   init_data_list_size (get_def_init_data def).
 
 Definition def_code_size (def: option gdef) :=
   code_size (get_def_instrs def).
 
+Definition defs_rodata_size (defs: list (option gdef)) :=
+  fold_right (fun def sz => def_rodata_size def + sz) 0 defs.
+             
 Definition defs_data_size (defs: list (option gdef)) :=
   fold_right (fun def sz => def_data_size def + sz) 0 defs.
 
 Definition defs_code_size (defs: list (option gdef)) :=
   fold_right (fun def sz => def_code_size def + sz) 0 defs.
 
+Lemma defs_rodata_size_cons: forall def defs,
+      defs_rodata_size (def :: defs) = (def_rodata_size def) + defs_rodata_size defs.
+Proof.
+  intros. unfold defs_rodata_size.
+  cbn. auto.
+Qed.
 
 Lemma defs_data_size_cons: forall def defs,
       defs_data_size (def :: defs) = (def_data_size def) + defs_data_size defs.
@@ -478,11 +538,11 @@ Proof.
   cbn. auto.
 Qed.
 
-Lemma symbtable_to_tree_cons: forall did cid tl dsz1 csz1 id def,
+Lemma symbtable_to_tree_cons: forall rdid did cid tl rdsz1 dsz1 csz1 id def,
     ~In id (get_symbentry_ids tl) ->
-    (symbtable_to_tree (get_symbentry did cid dsz1 csz1 id def :: tl)) ! id = Some (get_symbentry did cid dsz1 csz1 id def).
+    (symbtable_to_tree (get_symbentry rdid did cid rdsz1 dsz1 csz1 id def :: tl)) ! id = Some (get_symbentry rdid did cid rdsz1 dsz1 csz1 id def).
 Proof.
-  intros did cid tl dsz1 csz1 id def IN.
+  intros rdid did cid tl rdsz1 dsz1 csz1 id def IN.
   unfold symbtable_to_tree.
   cbn [symbtable_to_idlist map].
   rewrite get_symbentry_id.
@@ -494,9 +554,9 @@ Proof.
   rewrite list_map_compose. auto.
 Qed.
 
-Lemma symbtable_to_tree_tail: forall did cid tl dsz1 csz1 id id' def,
+Lemma symbtable_to_tree_tail: forall rdid did cid tl rdsz1 dsz1 csz1 id id' def,
     id <> id' ->
-    (symbtable_to_tree (get_symbentry did cid dsz1 csz1 id def :: tl)) ! id' =
+    (symbtable_to_tree (get_symbentry rdid did cid rdsz1 dsz1 csz1 id def :: tl)) ! id' =
     (symbtable_to_tree tl) ! id'.
 Proof.
   intros. unfold symbtable_to_tree.
@@ -506,43 +566,49 @@ Proof.
 Qed.
 
 
-Lemma update_code_data_size_inv: forall dsz1 csz1 def dsz2 csz2,
-          update_code_data_size dsz1 csz1 def = (dsz2, csz2) ->
-          dsz2 = dsz1 + def_data_size def /\
-          csz2 = csz1 + def_code_size def.
+Lemma update_section_size_inv: forall rdsz1 dsz1 csz1 id def rdsz2 dsz2 csz2,
+    update_section_size rdsz1 dsz1 csz1 id def = (rdsz2, dsz2, csz2) ->
+    rdsz2 = rdsz1 + def_rodata_size def /\
+    dsz2 = dsz1 + def_data_size def /\
+    csz2 = csz1 + def_code_size def.
 Proof.
-  intros dsz1 csz1 def dsz2 csz2 UPD.
-  unfold update_code_data_size in UPD. 
+  intros rdsz1 dsz1 csz1 id def rdsz2 dsz2 csz2 UPD.
+  unfold update_section_size in UPD. 
   destruct def. destruct g. destruct f.
-  - unfold def_data_size, def_code_size.
+  - unfold def_rodata_size, def_data_size, def_code_size.
     simpl in *. inv UPD. f_equal; omega.
-  - unfold def_data_size, def_code_size.
+  - unfold def_rodata_size, def_data_size, def_code_size.
     inv UPD. cbn. split; omega.
-  - destruct (gvar_init v) eqn:V.
-    + inv UPD. cbn. rewrite V. cbn. split; omega.
-    + destruct i; try (inv UPD; cbn; rewrite V; cbn; split; omega).
-      destruct l; try (inv UPD; cbn; rewrite V; cbn; split; omega). 
+  - destruct (gvar_init v) eqn:V0;destruct (gvar_readonly v) eqn:V1.
+    + inv UPD. cbn. rewrite V0. cbn. split; omega.
+    + inv UPD. cbn. rewrite V0. cbn. split; omega.
+    + destruct i; try (inv UPD; cbn; rewrite V0; rewrite V1; cbn; split; omega).
+      destruct l; try (inv UPD; cbn; rewrite V0; rewrite V1; cbn; split; omega).
+      inv UPD. cbn. rewrite V0. cbn. split. omega. omega.
+    + destruct i; try (inv UPD; cbn; rewrite V0; rewrite V1; cbn; split; omega).
+      destruct l; try (inv UPD; cbn; rewrite V0; rewrite V1; cbn; split; omega).
+      inv UPD. cbn. rewrite V0. cbn. split. omega. omega.
   - inv UPD. cbn. split; omega.
 Qed.
 
-
-Lemma acc_symb_tree_entry_some : forall did cid defs dsz1 csz1 dsz2 csz2 stbl id def,
+Lemma acc_symb_tree_entry_some : forall rdid did cid defs rdsz1 dsz1 csz1 rdsz2 dsz2 csz2 stbl id def,
     list_norepet (map fst defs) ->
-    fold_left (acc_symb did cid) defs ([], dsz1, csz1) = (stbl, dsz2, csz2) ->
+    fold_left (acc_symb rdid did cid) defs ([], rdsz1, dsz1, csz1) = (stbl, rdsz2, dsz2, csz2) ->
     (PTree_Properties.of_list defs)!id = Some def ->
     (symbtable_to_tree (rev stbl))!id 
-      = Some (get_symbentry did cid 
-                            (dsz1 + defs_data_size (defs_before id defs))
-                            (csz1 + defs_code_size (defs_before id defs))
+    = Some (get_symbentry rdid did cid
+             (rdsz1 + defs_rodata_size (defs_before id defs))           
+             (dsz1 + defs_data_size (defs_before id defs))
+             (csz1 + defs_code_size (defs_before id defs))
                             id
                             def).
 Proof.
   induction defs as [|def' defs].
   - cbn. inversion 1. subst. inv H. cbn. intros.
     rewrite PTree.gempty in H0. congruence.
-  - intros dsz1 csz1 dsz2 csz2 stbl id def NORPT ACC GET.
+  - intros rdsz1 dsz1 csz1 rdsz2 dsz2 csz2 stbl id def NORPT ACC GET.
     cbn in ACC. destruct def' as (id', def').
-    destr_in ACC. apply acc_symb_inv' in ACC.
+    destr_in ACC. destruct p. apply acc_symb_inv' in ACC.
     destruct ACC as (stbl' & EQ & ACC). subst.
     rewrite rev_app_distr.
     cbn [rev "++"].
@@ -561,31 +627,32 @@ Proof.
       { eapply PTree_Properties_of_list_tail_some; eauto. }
       rewrite symbtable_to_tree_tail; eauto.
       inv NORPT.
-      generalize (IHdefs _ _ _ _ _ _ _ H2 ACC GET').
+      generalize (IHdefs _ _ _ _ _ _ _ _ _ H2 ACC GET').
       intros SEQ. rewrite SEQ.
       setoid_rewrite defs_before_tail; auto.
       cbn [defs_data_size defs_code_size].
+      rewrite defs_rodata_size_cons.
       rewrite defs_data_size_cons.
       rewrite defs_code_size_cons.
-      generalize (update_code_data_size_inv _ _ _ _ _ Heqp).
+      generalize (update_section_size_inv _ _ _ _ _ _ _ _ Heqp).
       intros (EQ1 & EQ2); subst.
       f_equal. f_equal; omega.
 Qed.
 
 
-Lemma acc_symb_tree_entry_none : forall did cid defs dsz1 csz1 dsz2 csz2 stbl id,
-    fold_left (acc_symb did cid) defs ([], dsz1, csz1) = (stbl, dsz2, csz2) ->
+Lemma acc_symb_tree_entry_none : forall rdid did cid defs rdsz1 dsz1 csz1 rdsz2 dsz2 csz2 stbl id,
+    fold_left (acc_symb rdid did cid) defs ([], rdsz1, dsz1, csz1) = (stbl, rdsz2, dsz2, csz2) ->
     (PTree_Properties.of_list defs)!id = None ->
     (symbtable_to_tree (rev stbl))!id = None.
 Proof.
   induction defs as [|def defs].
-  - cbn. intros dsz1 csz1 dsz2 csz2 stbl id EQ GET.
+  - cbn. intros rdsz1 dsz1 csz1 rdsz2 dsz2 csz2 stbl id EQ GET.
     inv EQ. cbn.
     rewrite PTree.gempty. auto.
-  - intros dsz1 csz1 dsz2 csz2 stbl id FL GET.
+  - intros rdsz1 dsz1 csz1 rdsz2 dsz2 csz2 stbl id FL GET.
     destruct def as (id', def').
     cbn in FL.
-    destr_in FL.
+    destr_in FL. destruct p.
     apply acc_symb_inv' in FL.
     destruct FL as (stbl1' & EQ  & FL). subst.
     rewrite rev_app_distr. cbn [rev "++"].
@@ -601,10 +668,10 @@ Qed.
 
 
 Lemma acc_symb_tree_entry_some_inv:
-  forall (did cid : N) (defs : list (ident * option (globdef fundef unit)))
-    (dsz1 csz1 dsz2 csz2 : Z) (stbl : symbtable) (id : positive) e,
+  forall (rdid did cid : N) (defs : list (ident * option (globdef fundef unit)))
+    (rdsz1 dsz1 csz1 rdsz2 dsz2 csz2 : Z) (stbl : symbtable) (id : positive) e,
   list_norepet (map fst defs) ->
-  fold_left (acc_symb did cid) defs ([], dsz1, csz1) = (stbl, dsz2, csz2) ->
+  fold_left (acc_symb rdid did cid) defs ([], rdsz1, dsz1, csz1) = (stbl, rdsz2, dsz2, csz2) ->
   (symbtable_to_tree (rev stbl)) ! id = Some e ->
   exists def, (PTree_Properties.of_list defs) ! id = Some def.
 Proof.
@@ -615,7 +682,7 @@ Proof.
   - intros until e.
     intros NORPT ACC ST. inv NORPT.
     cbn in ACC. destruct def as (id', def).
-    destr_in ACC.
+    destr_in ACC. destruct p.
     apply acc_symb_inv' in ACC.
     destruct ACC as (stbl1 & EQ & ACC). subst.
     rewrite rev_app_distr in ST. cbn [rev "++"] in ST.
@@ -624,38 +691,39 @@ Proof.
       eapply PTree_Properties.of_list_dom; eauto.
       cbn. auto.
     + erewrite symbtable_to_tree_tail in ST; eauto.
-      generalize (IHdefs _ _ _ _ _ _ _ H2 ACC ST).
+      generalize (IHdefs _ _ _ _ _ _ _ _ _ H2 ACC ST).
       intros (def1 & GET1).
       rewrite PTree_Properties_of_list_tail; eauto.
 Qed.
 
-Definition symbtable_entry_equiv_sizes stbl dsz1 csz1 defs1 :=
-  forall did cid dsz3 csz3 id def,
-    In (get_symbentry did cid dsz3 csz3 id def) stbl ->
-    get_symbentry did cid dsz3 csz3 id def =
-    get_symbentry did cid 
+Definition symbtable_entry_equiv_sizes stbl rdsz1 dsz1 csz1 defs1 :=
+  forall rdid did cid rdsz3 dsz3 csz3 id def,
+    In (get_symbentry rdid did cid rdsz3 dsz3 csz3 id def) stbl ->
+    get_symbentry rdid did cid rdsz3 dsz3 csz3 id def =
+    get_symbentry rdid did cid
+                  (rdsz1 + defs_rodata_size (defs_before id defs1))
                   (dsz1 + defs_data_size (defs_before id defs1))
                   (csz1 + defs_code_size (defs_before id defs1))
                   id def.
 
-Lemma symbtable_entry_equiv_sizes_app_comm: forall l1 l2 dsz csz defs,
-    symbtable_entry_equiv_sizes (l1 ++ l2) dsz csz defs ->
-    symbtable_entry_equiv_sizes (l2 ++ l1) dsz csz defs.
+Lemma symbtable_entry_equiv_sizes_app_comm: forall l1 l2 rdsz dsz csz defs,
+    symbtable_entry_equiv_sizes (l1 ++ l2) rdsz dsz csz defs ->
+    symbtable_entry_equiv_sizes (l2 ++ l1) rdsz dsz csz defs.
 Proof.
-  intros l1 l2 dsz csz defs SE.
+  intros l1 l2 rdsz dsz csz defs SE.
   red. intros; eapply SE; eauto.
   rewrite in_app in *. inv H. 
   right; eauto.
   left; eauto.
 Qed.
 
-Lemma symbtable_entry_equiv_sizes_app: forall l1 l2 dsz csz defs,
-    symbtable_entry_equiv_sizes l1 dsz csz defs ->
-    symbtable_entry_equiv_sizes l2 dsz csz defs ->
-    symbtable_entry_equiv_sizes (l1 ++ l2) dsz csz defs.
+Lemma symbtable_entry_equiv_sizes_app: forall l1 l2 rdsz dsz csz defs,
+    symbtable_entry_equiv_sizes l1 rdsz dsz csz defs ->
+    symbtable_entry_equiv_sizes l2 rdsz dsz csz defs ->
+    symbtable_entry_equiv_sizes (l1 ++ l2) rdsz dsz csz defs.
 Proof.
-  intros l1 l2 dsz csz defs SE1 SE2.
-  red. intros did cid dsz3 csz3 id def IN.
+  intros l1 l2 rdsz dsz csz defs SE1 SE2.
+  red. intros rdid did cid rdsz3 dsz3 csz3 id def IN.
   rewrite in_app in IN. 
   destruct IN as [IN | IN].
   - eapply SE1; eauto.
@@ -663,24 +731,27 @@ Proof.
 Qed.
 
 Lemma acc_symb_size':
-  forall (d_id c_id : N) (defs : list (ident * option (globdef fundef unit)))
-    (s1 s2 : symbtable) (dsz1 csz1 dsz2 csz2 : Z),
-    fold_left (acc_symb d_id c_id) defs (s1, dsz1, csz1) = (s2, dsz2, csz2) ->
+  forall (rd_id r_id c_id : N) (defs : list (ident * option (globdef fundef unit)))
+    (s1 s2 : symbtable) (rdsz1 dsz1 csz1 rdsz2 dsz2 csz2 : Z),
+    fold_left (acc_symb rd_id r_id c_id) defs (s1, rdsz1, dsz1, csz1) = (s2, rdsz2, dsz2, csz2) ->
+    rdsz2 = rdsz1 + defs_rodata_size (map snd defs) /\
     dsz2 = dsz1 + defs_data_size (map snd defs) /\
     csz2 = csz1 + defs_code_size (map snd defs).
 Proof.
   induction defs as [|def defs].
   - cbn. inversion 1. split; omega.
-  - intros s1 s2 dsz1 csz1 dsz2 csz2 ACC.
+  - intros s1 s2 rdsz1 dsz1 csz1 rdsz2 dsz2 csz2 ACC.
     cbn in ACC. destruct def as (id, def). 
     cbn [map snd].
     rewrite defs_code_size_cons.
     rewrite defs_data_size_cons.
-    destr_in ACC.
-    generalize (update_code_data_size_inv _ _ _ _ _ Heqp).
-    intros (EQ1 & EQ2). subst.
+    rewrite defs_rodata_size_cons.
+    destr_in ACC. destruct p.
+    generalize (update_section_size_inv _ _ _ _ _ _ _ _ Heqp).
+    intros (EQ1 & EQ2 & EQ3). subst.
     apply IHdefs in ACC. 
-    destruct ACC. subst; omega.
+    destruct ACC. destruct H0.
+    subst; omega.
 Qed.
 
 Lemma acc_instrs_size: forall defs,
@@ -1017,18 +1088,18 @@ Proof.
 Qed.
 
 Lemma gen_symb_table_only_internal_symbol_aux: 
-  forall did cid defs stbl dz1 cz1 dz2 cz2 id def,
+  forall rdid did cid defs stbl rdz1 dz1 cz1 rdz2 dz2 cz2 id def,
     list_norepet (map fst defs) ->
     is_def_internal is_fundef_internal def = true ->
-    fold_left (acc_symb did cid) defs ([], dz1, cz1) = (stbl, dz2, cz2) ->
+    fold_left (acc_symb rdid did cid) defs ([], rdz1, dz1, cz1) = (stbl, rdz2, dz2, cz2) ->
     In (id, def) defs ->
     only_internal_symbol id (rev stbl).
 Proof.
   induction defs as [|def defs].
   - cbn. intros. contradiction.
-  - intros stbl dz1 cz1 dz2 cz2 id def1 NORPT INT ACC IN. 
+  - intros stbl rdz1 dz1 cz1 rdz2 dz2 cz2 id def1 NORPT INT ACC IN. 
     inv NORPT. cbn in ACC. destruct def as (id1, def).
-    destr_in ACC.
+    destr_in ACC. destruct p.
     apply acc_symb_inv' in ACC.
     destruct ACC as (stbl1' & EQ & ACC). subst.
     rewrite rev_app_distr. cbn.
@@ -1051,17 +1122,17 @@ Qed.
       
 
 Lemma gen_symb_table_only_internal_symbol: 
-  forall did cid defs stbl dz cz id def,
+  forall rdid did cid defs stbl rdz dz cz id def,
     list_norepet (map fst defs) ->
     is_def_internal is_fundef_internal def = true ->
-    gen_symb_table did cid defs = (stbl, dz, cz) ->
+    gen_symb_table rdid did cid defs = (stbl, rdz, dz, cz) ->
     In (id, def) defs ->
     only_internal_symbol id stbl.
 Proof.
   intros until def.
   intros NORPT INT GS IN.
   unfold gen_symb_table in GS. destr_in GS.
-  destruct p. inv GS.
+  destruct p. destruct p. inv GS.
   eapply gen_symb_table_only_internal_symbol_aux; eauto.
 Qed.
 
@@ -1176,10 +1247,10 @@ Lemma gen_symb_map_internal_block_range: forall stbl e b ofs i,
     list_norepet (get_symbentry_ids stbl) ->
     is_symbentry_internal e = true ->
     symbentry_secindex e = secindex_normal i ->
-    (i < 3)%N ->
+    (i < 4)%N ->
     In e stbl ->
     (gen_symb_map stbl) ! (symbentry_id e) = Some (b, ofs) ->
-    (b < 3)%positive.
+    (b < 4)%positive.
 Proof.
   induction stbl as [|e' stbl].
   - cbn. intros. contradiction.
@@ -1232,5 +1303,3 @@ Proof.
     eapply IHdefs; eauto.
     eapply Z.divide_add_r; eauto.
 Qed.
-*)
-(***** Remove Proofs By Chris End ******)
