x86/AsmFloatLiteralSep.v
@@ -1,17 +1,17 @@
-(* *******************  *)
-(* Author: Yuting Wang  *)
-(* Date:   Dec 2, 2019 *)
-(* *******************  *)
+(* ******************** *)
+(* Author: Zhenguo Yin  *)
+(* Date:   Sep 21, 2020 *)
+(* ******************** *)
 
 Require Import Coqlib Errors.
 Require Import Integers Floats AST Linking.
 Require Import Values Memory Events Globalenvs Smallstep.
 Require Import Op Locations Mach Conventions Asm RealAsm.
-Require Import PadInitData PadInitDataproof.
+Require Import AsmFloatLiteral AsmFloatLiteralproof.
 Import ListNotations.
 
 Instance TransfPermuteOrderedLink2 
-  : TransfLink PadInitDataproof.match_prog.
+  : TransfLink AsmFloatLiteralproof.match_prog.
 Proof.
   red. unfold match_prog.
 Admitted.
