x86/Jumptablegenproof.v
@@ -1,0 +1,55 @@
+(* ******************** *)
+(* Author: Zhenguo Yin  *)
+(* Date:   Sep 21, 2020 *)
+(* ******************** *)
+
+Require Import Coqlib Errors.
+Require Import Integers Floats AST Linking.
+Require Import Values Memory Events Globalenvs Smallstep.
+Require Import Op Locations Mach Conventions Asm RealAsm.
+Require Import RelocProgram RelocProgSemantics.
+Require Import Jumptablegen.
+Import ListNotations.
+Require AsmFacts.
+
+Definition match_prog (p tp:program) :=
+  exists tp',
+    transf_program p = OK tp' /\
+    prog_public tp = prog_public tp' /\
+    prog_main tp = prog_main tp' /\
+    prog_strtable tp = prog_strtable tp' /\
+    prog_reloctables tp = prog_reloctables tp' /\
+    prog_senv tp = prog_senv tp'.
+
+Lemma transf_program_match:
+  forall p tp, transf_program p = OK tp -> match_prog p tp.
+Proof.
+  unfold match_prog. intros. exists tp; intuition.
+Qed.
+
+Require Import RelocLinking.
+Instance jumptablegen_transflink : @TransfLink _ _ RelocLinking.Linker_reloc_prog RelocLinking.Linker_reloc_prog match_prog.
+Proof.
+  Admitted.
+
+Section PRESERVATION.
+  Existing Instance inject_perm_all.
+Context `{external_calls_prf: ExternalCalls}.
+
+Local Existing Instance mem_accessors_default.
+
+Variable prog: RelocProgram.program.
+Variable tprog: RelocProgram.program.
+
+Let ge := RelocProgSemantics.globalenv prog.
+Let tge := RelocProgSemantics.globalenv tprog.
+
+Hypothesis TRANSF: match_prog prog tprog.
+
+Lemma transf_program_correct:
+  forall rs, forward_simulation (RelocProgSemantics.semantics prog rs) (RelocProgSemantics.semantics tprog rs).
+Proof.
+Admitted.
+
+
+End PRESERVATION.
